bench/compile-and-run.sh
@@ -11,9 +11,9 @@ mv ../../fscq/fscq15/src/fuse ./fs/CfscqFs
 mv ../../fscq/fscq15/src/mkfs ./fs/CfscqMkfs
 
 ./compile-sources.sh
-./run-confs.sh 10 $1
-./run-cfscq.sh 10 $1
-./run-sfscq.sh 10 $1
-
+sudo rm -rf results
+sudo ./run-confs.sh $2 $1
+sudo ./run-cfscq.sh $2 $1
+sudo ./run-sfscq.sh $2 $1
 
 ./get-stats.sh
